src/ghost/trace.fst
@@ -17,90 +17,52 @@
 
 module Tesseract.Ghost.Trace
 
-   type step_fn (ev_t: Type) (st_t: Type) = 
-      ev_t -> st_t -> Tot st_t
+   type step_g (state_t: Type) (event_t: Type) = 
+      | Init: state: state_t -> step_g state_t event_t
+      | Next: state: state_t -> event: event_t -> step_g state_t event_t
 
-   type _trace (ev_t: Type) (st_t: Type) =
+   type transform_g (state_t: Type) (event_t: Type) =
+      state_t -> event_t -> Tot state_t
+
+   type trace_g (state_t: Type) (event_t: Type) =
       {
-         log: Seq.seq (ev_t * st_t);
-         step: step_fn ev_t st_t;
-         initst: st_t
+         event_log: Seq.seq_g event_t;
+         transform: transform_g state_t event_t;
+         state0: state_t
       }
 
-   type is_safe: #ev_t: Type -> #st_t: Type -> _trace ev_t st_t -> Type =
-      fun (ev_t: Type) (st_t: Type) (tr: _trace ev_t st_t) ->
-         // empty logs are safe.
-         (0 = (Seq.length tr.log))
-         // the first entry of the log must be the result of the first event applied to the initialization state.
-         \/ ((match Seq.nth tr.log 0 with
-               | (e, s') ->
-                  s' = tr.step e tr.initst)
-            // all remaining steps are derived similarly from the state in the previous log entry.
-            /\ (forall i.
-                  0 < i && i < (Seq.length tr.log)
-                  ==>
-                     (match Seq.nth tr.log (i - 1) with
-                        | (_, s) ->
-                           match Seq.nth tr.log i with
-                              | (e, s') ->
-                                 s' = tr.step e s)))
-
-   type trace (ev_t: Type) (st_t: Type) =
-      tr: _trace ev_t st_t{is_safe tr}
-
-   val new: #ev_t: Type -> #st_t: Type -> step_fn ev_t st_t -> st_t -> Tot (trace ev_t st_t)
-   let new (ev_t: Type) (st_t: Type) fn st0 = 
+   val init: 
+      #state_t: Type -> #event_t: Type -> 
+      transform_g state_t event_t -> state_t -> Tot (trace_g state_t event_t)
+   let init (state_t: Type) (event_t: Type) f s = 
       {
-         log = Seq.empty;
-         step = fn;
-         initst = st0
+         event_log = Seq.empty;
+         transform = f;
+         state0 = s
       }
 
-   val log: #ev_t: Type -> #st_t: Type -> trace ev_t st_t -> Tot (Seq.seq (ev_t * st_t))
-   let log (ev_t: Type) (st_t: Type) trc =
-      trc.log
-
-   val initst: #ev_t: Type -> #st_t: Type -> trace ev_t st_t -> Tot st_t
-   let initst (ev_t: Type) (st_t: Type) tr =
-      tr.initst
-   
-   val curst: #ev_t: Type -> #st_t: Type -> trace ev_t st_t -> Tot st_t
-   let curst (ev_t: Type) (st_t: Type) tr =
-      if 0 = Seq.length (log tr) then
-         initst tr
-      else
-         match Seq.last (log tr) with
-            | (_, s) ->
-               s
-
-   val now: #ev_t: Type -> #st_t: Type -> trace ev_t st_t -> Tot st_t
-   let now (ev_t: Type) (st_t: Type) tr =
-      if 0 = Seq.length tr.log then
-         initst tr
-      else
-         match Seq.last tr.log with
-            | (_, s) ->
-               s
-
-   val step: #ev_t: Type -> #st_t: Type -> trace ev_t st_t -> ev_t -> Tot (trace ev_t st_t)
-   let step (ev_t: Type) (st_t: Type) tr ev =
-      let 
-         state =
-            // todo: f* doesn't see that s = Seq.empty <==> 0 = Seq.length s. 
-            // this seems like a good opportunity for a lemma related to Seq.empty.
-            // todo: would functional extensionality help somehow here?
-            //if tr.log = Seq.empty then
-            if 0 = Seq.length tr.log then
-               tr.initst
-            else
-               match Seq.last tr.log with
-                  | (_, s) ->
-                     s
+   val steps:
+      #state_t: Type -> #event_t: Type -> 
+      trace_g state_t event_t -> Tot (Seq.seq_g (step_g state_t event_t))
+   let steps (state_t: Type) (event_t: Type) trace =
+      let head = Seq.single (Init trace.state0) in
+      let tail =
+         Seq.foldl
+            (fun (accum: Seq.seq_g (step_g state_t event_t){0 < Seq.length accum}) event ->
+               let step = 
+                  (let state = 
+                     match Seq.last accum with
+                        | Init s ->
+                           s
+                        | Next s _ ->
+                           s
+                  in
+                     Next (trace.transform state event) event)
+               in
+                  Seq.append accum step)
+            head
+            trace.event_log
       in
-         {
-            log = Seq.append tr.log (ev, tr.step ev state);
-            step = tr.step;
-            initst = tr.initst
-         }
+         Seq.concat head tail
 
 // $vim-fst:32: vim:set sts=3 sw=3 et ft=fstar:,$
